theories/examples/soc/soc_enclave_spec.v
@@ -1,30 +1,30 @@
 From iris.proofmode Require Import proofmode.
 From cap_machine Require Import rules logrel fundamental.
 From cap_machine Require Import proofmode.
-From cap_machine Require Import trusted_compute_code.
+From cap_machine Require Import soc_code.
 Open Scope Z_scope.
 
 
-Section trusted_compute_enclave.
+Section soc_enclave.
   Context {Σ:gFunctors} {ceriseg:ceriseG Σ} {sealsg: sealStoreG Σ}
           {nainv: logrel_na_invs Σ}
           {reservedaddresses : ReservedAddresses}
           `{MP: MachineParameters}.
-  Context {TC : TrustedCompute}.
+  Context {SOC : SecureOutsourcedCompute}.
 
-  Lemma tc_enclave_contract :
-    ⊢ custom_enclave_contract (enclaves_map := contract_tc_enclaves_map).
+  Lemma soc_enclave_contract :
+    ⊢ custom_enclave_contract (enclaves_map := contract_soc_enclaves_map).
   Proof.
     iLöb as "IH".
     rewrite -/custom_enclave_contract.
     iEval (rewrite /custom_enclave_contract).
     iIntros (I b e v b' e' a' v' enclave_data ot ce
       Hcode_ce Hot HIhash Hb He)
-      "(#Hcustoms_inv & #Htc_inv & #HPenc & #HPsign)".
+      "(#Hcustoms_inv & #Hsoc_inv & #HPenc & #HPsign)".
     assert (e = (b ^+ (length (code ce) + 1))%a) as -> by solve_addr+He.
     simplify_map_eq.
-    rewrite /tcenclaves_map in Hcode_ce.
-    replace ((λ w : Word, word_to_lword w v) <$> code ce) with trusted_compute_enclave_lcode.
+    rewrite /soc_enclaves_map in Hcode_ce.
+    replace ((λ w : Word, word_to_lword w v) <$> code ce) with soc_enclave_lcode.
     2:{ simplify_map_eq. cbn. rewrite /encodeInstrWL. done. }
     simplify_map_eq.
     rewrite -H; clear H.
@@ -32,12 +32,12 @@ Section trusted_compute_enclave.
     iIntros (lregs); iNext ; iModIntro.
     iIntros "([%Hfullmap #Hinterp_map] & Hrmap & Hna)".
     rewrite /interp_conf.
-    iMod (na_inv_acc with "Htc_inv Hna") as "(>[Htc_code Htc_data]  & Hna & Hclose)"; [solve_ndisj ..|].
+    iMod (na_inv_acc with "Hsoc_inv Hna") as "(>[Hsoc_code Hsoc_data]  & Hna & Hclose)"; [solve_ndisj ..|].
     rewrite /registers_mapsto.
     iExtract "Hrmap" PC as "HPC".
-    remember tc_addr as pc_b in |- * at 7.
-    remember (tc_addr ^+ (20%nat + 1))%a as pc_e in |- * at 4.
-    assert (SubBounds pc_b pc_e tc_addr (tc_addr ^+ (20%nat + 1))%a) by (subst; solve_addr).
+    remember soc_addr as pc_b in |- * at 7.
+    remember (soc_addr ^+ (20%nat + 1))%a as pc_e in |- * at 4.
+    assert (SubBounds pc_b pc_e soc_addr (soc_addr ^+ (20%nat + 1))%a) by (subst; solve_addr).
 
     (* Prepare the necessary resources *)
     (* Registers *)
@@ -84,75 +84,75 @@ Section trusted_compute_enclave.
       done.
     }
     (* Code memory *)
-    iDestruct (region_mapsto_cons with "Htc_code") as "[Htc_addr Htc_code]"; last iFrame.
-    { transitivity (Some (tc_addr ^+ 1)%a); auto ; try solve_addr. }
+    iDestruct (region_mapsto_cons with "Hsoc_code") as "[Hsoc_addr Hsoc_code]"; last iFrame.
+    { transitivity (Some (soc_addr ^+ 1)%a); auto ; try solve_addr. }
     { solve_addr. }
-    iAssert (codefrag (tc_addr ^+ 1%nat)%a v trusted_compute_enclave_lcode)
-      with "[Htc_code]" as "Htc_code".
+    iAssert (codefrag (soc_addr ^+ 1%nat)%a v soc_enclave_lcode)
+      with "[Hsoc_code]" as "Hsoc_code".
     {
       rewrite /codefrag /=.
-      by replace ((tc_addr ^+ 1%nat) ^+ 20%nat)%a with (tc_addr ^+ 21%nat)%a by solve_addr.
+      by replace ((soc_addr ^+ 1%nat) ^+ 20%nat)%a with (soc_addr ^+ 21%nat)%a by solve_addr.
     }
-    codefrag_facts "Htc_code".
+    codefrag_facts "Hsoc_code".
 
     (* Data memory *)
     iAssert (⌜ (b' < e')%a ⌝)%I as "%Hb'".
     {
-      iDestruct (big_sepL2_length with "Htc_data") as "%Htc_data_len".
-      rewrite map_length /= in Htc_data_len.
+      iDestruct (big_sepL2_length with "Hsoc_data") as "%Hsoc_data_len".
+      rewrite map_length /= in Hsoc_data_len.
       iPureIntro.
-      clear - Htc_data_len.
+      clear - Hsoc_data_len.
       destruct (decide (b' < e')) as [He' | He']; cycle 1.
-      - rewrite finz_seq_between_empty in Htc_data_len; last solve_addr.
+      - rewrite finz_seq_between_empty in Hsoc_data_len; last solve_addr.
         cbn in * ; discriminate.
       - done.
     }
-    iDestruct (region_mapsto_cons with "Htc_data") as "[Htc_keys Htc_data]"; last iFrame.
+    iDestruct (region_mapsto_cons with "Hsoc_data") as "[Hsoc_keys Hsoc_data]"; last iFrame.
     { transitivity (Some (b' ^+ 1)%a); auto ; try solve_addr. }
     { solve_addr. }
 
 
     (* Prove the spec *)
-    iInstr "Htc_code". (* Mov r_t1 PC *)
-    iInstr "Htc_code". (* Lea r_t1 (-1)%Z *)
-    transitivity (Some tc_addr); auto ; solve_addr.
+    iInstr "Hsoc_code". (* Mov r_t1 PC *)
+    iInstr "Hsoc_code". (* Lea r_t1 (-1)%Z *)
+    transitivity (Some soc_addr); auto ; solve_addr.
 
-    iInstr "Htc_code". (* Load r_t1 r_t1 *)
+    iInstr "Hsoc_code". (* Load r_t1 r_t1 *)
     apply le_addr_withinBounds; solve_addr.
-    iInstr "Htc_code". (* GetB r_t2 r_t1 *)
-    iInstr "Htc_code". (* GetA r_t3 r_t1 *)
-    iInstr "Htc_code". (* Sub r_t2 r_t2 r_t3 *)
-    iInstr "Htc_code". (* Lea r_t1 r_t2 *)
+    iInstr "Hsoc_code". (* GetB r_t2 r_t1 *)
+    iInstr "Hsoc_code". (* GetA r_t3 r_t1 *)
+    iInstr "Hsoc_code". (* Sub r_t2 r_t2 r_t3 *)
+    iInstr "Hsoc_code". (* Lea r_t1 r_t2 *)
     transitivity (Some b'); auto ; solve_addr.
 
-    iInstr "Htc_code". (* Load r_t1 r_t1 *)
+    iInstr "Hsoc_code". (* Load r_t1 r_t1 *)
     apply le_addr_withinBounds; solve_addr.
-    iInstr "Htc_code". (* GetE r_t3 r_t1 *)
-    iInstr "Htc_code". (* Sub r_t3 r_t2 1 *)
+    iInstr "Hsoc_code". (* GetE r_t3 r_t1 *)
+    iInstr "Hsoc_code". (* Sub r_t3 r_t2 1 *)
     replace (((ot ^+ 2)%f - 1)) with (ot + 1) by solve_finz.
-    iInstr "Htc_code". (* Subseg r_t1 r_t2 r_t3 *)
+    iInstr "Hsoc_code". (* Subseg r_t1 r_t2 r_t3 *)
     transitivity (Some (ot ^+1)%ot); auto ; solve_finz.
     apply isWithin_of_le; solve_finz.
 
-    iInstr "Htc_code". (* Mov r_t2 PC *)
-    iInstr "Htc_code". (* GetA r_t3 r_t2 *)
-    iInstr "Htc_code". (* Sub r_t3 42 r_t3 *)
+    iInstr "Hsoc_code". (* Mov r_t2 PC *)
+    iInstr "Hsoc_code". (* GetA r_t3 r_t2 *)
+    iInstr "Hsoc_code". (* Sub r_t3 42 r_t3 *)
 
     assert (
-        ((tc_addr ^+ 1) ^+ 11 + (42 - ((tc_addr ^+ 1) ^+ 11)))%a = Some f42)
+        ((soc_addr ^+ 1) ^+ 11 + (42 - ((soc_addr ^+ 1) ^+ 11)))%a = Some f42)
       as Hoffset by (by rewrite finz_incr_minus_id).
-    iInstr "Htc_code". (* Lea r_t2 r_t3 *)
-    iInstr "Htc_code". (* Restrict r_t2 (encodePerm O) *)
+    iInstr "Hsoc_code". (* Lea r_t2 r_t3 *)
+    iInstr "Hsoc_code". (* Restrict r_t2 (encodePerm O) *)
     by rewrite decode_encode_perm_inv.
     rewrite decode_encode_perm_inv.
-    iInstr "Htc_code". (* Lea r_t1 1 *)
+    iInstr "Hsoc_code". (* Lea r_t1 1 *)
     transitivity (Some (ot ^+ 1)%ot); auto ; solve_finz.
-    iInstr "Htc_code". (* Seal r_t2 r_t2 r_t1 *)
+    iInstr "Hsoc_code". (* Seal r_t2 r_t2 r_t1 *)
     by cbn.
     apply le_addr_withinBounds; solve_finz.
 
     (* Restrict r_t1 (encodeSealPerms (false, true)) *)
-    iInstr_lookup "Htc_code" as "Hi" "Htc_code".
+    iInstr_lookup "Hsoc_code" as "Hi" "Hsoc_code".
     wp_instr.
     iApply (wp_restrict_success_z_sr with "[HPC Hr1 Hi]")
     ; try iFrame
@@ -160,13 +160,13 @@ Section trusted_compute_enclave.
     ; repeat (rewrite decode_encode_seal_perms_inv)
     ; try done.
     iNext; iIntros "(HPC & Hi & Hr1)".
-    all: wp_pure; iInstr_close "Htc_code".
+    all: wp_pure; iInstr_close "Hsoc_code".
 
     (* Prepare the jump to adversary: prove all registers contain safe values *)
     iAssert (interp w0) as "Hinterp_w0".
     { iApply "Hinterp_map" ; eauto; done. }
 
-    iAssert (interp (LSealedCap (ot ^+ 1)%f O tc_addr (tc_addr ^+ 21%nat)%a f42 v))
+    iAssert (interp (LSealedCap (ot ^+ 1)%f O soc_addr (soc_addr ^+ 21%nat)%a f42 v))
       as "Hinterp_sealed42".
     {
       iClear "Hinterp_map Hinterp_w0".
@@ -197,18 +197,18 @@ Section trusted_compute_enclave.
       iModIntro.
       by iApply custom_enclave_contract_inv.
     }
-    iInstr "Htc_code". (* Jmp r_t0 *)
+    iInstr "Hsoc_code". (* Jmp r_t0 *)
 
     (* Close the opened invariant *)
-    iDestruct (region_mapsto_cons with "[Htc_addr Htc_code]") as "Htc_code"
+    iDestruct (region_mapsto_cons with "[Hsoc_addr Hsoc_code]") as "Hsoc_code"
     ; try iFrame
     ; try solve_addr.
-    iDestruct (region_mapsto_cons with "[Htc_keys Htc_data]") as "Htc_data"
+    iDestruct (region_mapsto_cons with "[Hsoc_keys Hsoc_data]") as "Hsoc_data"
     ; try iFrame
     ; try solve_addr.
-    replace ((tc_addr ^+ 1%nat)%a ^+ length trusted_compute_enclave_lcode)%a with
-      (tc_addr ^+ 21%nat)%a by solve_addr.
-    iMod ("Hclose" with "[$Hna $Htc_code $Htc_data]") as "Hna".
+    replace ((soc_addr ^+ 1%nat)%a ^+ length soc_enclave_lcode)%a with
+      (soc_addr ^+ 21%nat)%a by solve_addr.
+    iMod ("Hclose" with "[$Hna $Hsoc_code $Hsoc_data]") as "Hna".
     (* Wrap up the registers *)
     iDestruct (big_sepM_insert _ _ r_t0 with "[$Hrmap $Hr0]") as "Hrmap".
     { do 3 ( rewrite lookup_delete_ne //) ; by rewrite lookup_delete. }
@@ -223,8 +223,8 @@ Section trusted_compute_enclave.
     { do 0 ( rewrite lookup_delete_ne //) ; by rewrite lookup_delete. }
     do 0 (rewrite -delete_insert_ne //=); rewrite insert_delete_insert.
 
-    set ( rmap' := <[r_t3:=LInt (42 - ((tc_addr ^+ 1) ^+ 11)%a)]>
-                            (<[r_t2:=LSealedCap (ot ^+ 1)%f O tc_addr (tc_addr ^+ 21%nat)%a f42 v]>
+    set ( rmap' := <[r_t3:=LInt (42 - ((soc_addr ^+ 1) ^+ 11)%a)]>
+                            (<[r_t2:=LSealedCap (ot ^+ 1)%f O soc_addr (soc_addr ^+ 21%nat)%a f42 v]>
                                (<[r_t1:=LSealRange (false, true) (ot ^+ 1)%f (ot ^+ 2)%f (ot ^+ 1)%f]>
                                   (<[r_t0:=w0]> (delete PC lregs))))).
     iAssert ([∗ map] k↦y ∈ rmap', k ↦ᵣ y ∗ interp y)%I with "[Hrmap]" as "Hrmap".
@@ -251,4 +251,4 @@ Section trusted_compute_enclave.
     }
     iApply ("Hjmp" with "[]") ; eauto ; iFrame.
   Qed.
-End trusted_compute_enclave.
+End soc_enclave.
